\newpage		
	\section*{}
	\textbf{Task}\\
	Prove the equality:
	\begin{gather*}
		\sum\limits_{k=0}^{n} {{n}\choose{k}}^2 = {{2n}\choose{n}}
	\end{gather*}
	\textbf{Solution}\\
	We know that
	\begin{gather*}
		{{n}\choose{k}} = {{n}\choose{n-k}}
	\end{gather*}
	Then
	\begin{gather*}
		\sum\limits_{k=0}^{n} {{n}\choose{k}}^2 = 
		\sum\limits_{k=0}^{n} {{n}\choose{k}}{{n}\choose{n-k}}
	\end{gather*}
	Then we can see that this is the same as choosing $n-k$ objectsfrom the set of power $n$ and $k$ from the other set with the same size. Then, considering the sum of ${{n}\choose{k}}{{n}\choose{n-k}}$ for all possible k, we get the number of ways to select $n$ objects from a set of size $2n$. 